theories/heap_lang/adequacy.v
@@ -1,25 +1,29 @@
 From iris.program_logic Require Export weakestpre adequacy.
 From iris.algebra Require Import auth.
+From iris_time Require Import Auth_nat.
 From iris_time.heap_lang Require Import proofmode notation.
 From iris.proofmode Require Import proofmode.
 Set Default Proof Using "Type".
 
 Class heapGpreS Σ := HeapGpreS {
   #[global] heap_preG_iris :: invGpreS Σ;
-  #[global] heap_preG_heap :: gen_heapGpreS loc val Σ
+  #[global] heap_preG_heap :: gen_heapGpreS loc val Σ;
+  #[local] heap_preG_nat :: inG Σ (authR natUR);
 }.
 
-Definition heapΣ : gFunctors := #[invΣ; gen_heapΣ loc val].
+Definition heapΣ : gFunctors := #[invΣ; gen_heapΣ loc val; GFunctor (authR natUR)].
 Global Instance subG_heapPreG {Σ} : subG heapΣ Σ → heapGpreS Σ.
 Proof. solve_inG. Qed.
 
 Definition heap_adequacy Σ `{heapGpreS Σ} s e σ φ :
-  (∀ `{heapGS Σ}, ⊢ WP e @ s; ⊤ {{ v, ⌜φ v⌝ }}) →
+  (∀ `{heapGS Σ}, TC (σ.(tick_counter)) ⊢ WP e @ s; ⊤ {{ v, ⌜φ v⌝ }}) →
   adequate s e σ (λ v _, φ v).
 Proof.
   intros Hwp; eapply (wp_adequacy _ _); iIntros (??) "".
-  iMod (gen_heap_init σ) as (?) "[Hh _]".
+  iMod (gen_heap_init σ.(heap)) as (?) "[Hh _]".
+  iMod (auth_nat_alloc σ.(tick_counter)) as (γ) "[Htc● Htc◯]".
   iModIntro.
-  iExists (λ σ κs, (gen_heap_interp σ)%I), (λ _, True%I). iFrame.
-  iApply (Hwp (HeapGS _ _ _)).
+  iExists (λ σ κs, (gen_heap_interp σ.(heap) ∗ own γ (●nat σ.(tick_counter)))%I),
+    (λ _, True%I). iFrame.
+  iApply (Hwp (HeapGS _ _ _ _ _)). iFrame.
 Qed.
