theories/Simulation.v
@@ -13,35 +13,11 @@ Implicit Type m n : nat.
 Implicit Type φ : val → Prop.
 
 
-
-(* Our definition of “tick” will depend on a location. This is made a typeclass
- * so as to be inferred automatically. *)
-Class TickCounter := { tick_counter : loc }.
-Notation "S« σ , n »" := (<[tick_counter := LitV (LitInt n%nat)]> (translationS σ%V)).
+Notation "S« σ , n »" := (state_set_tick_counter n (translationS σ%V)).
 (* Notation "« σ , n »" := (<[ℓ := LitV (LitInt n%nat)]> (translationS σ%V)) (only printing). *)
-Local Notation ℓ := tick_counter.
-
 
 (* This whole file is parameterized by a “runtime_error” value: *)
 Section Simulation.
-Context (runtime_error : val).
-
-
-
-(*
- * Definition of “tick”
- *)
-
-Local Instance generic_tick {Hloc : TickCounter} : Tick :=
- (rec: "tick" "x" :=
-    let: "k" := ! #ℓ in
-    if: "k" ≤ #0 then
-      runtime_error #()
-    else if: CAS #ℓ "k" ("k" - #1) then
-      "x"
-    else
-      "tick" "x")%V.
-
 
 (*
  * Operational behavior of “tick”
@@ -49,40 +25,17 @@ Local Instance generic_tick {Hloc : TickCounter} : Tick :=
 
 Section Tick_exec.
 
-  Context {Hloc : TickCounter}.
-
   Lemma exec_tick_success n v σ :
-    prim_exec  (tick v) (<[ℓ := #(S n)]> σ)  v (<[ℓ := #n]> σ)  [].
+    prim_exec  (Tick v) (state_set_tick_counter (S n) σ)  v (state_set_tick_counter n σ)  [].
   Proof.
-    remember (Z.of_nat (S n)) as Sn.
-    unlock tick generic_tick.
-    eapply prim_exec_cons_nofork. (* Initial β-redex *)
-    { by prim_step. }
-    simpl. eapply prim_exec_cons_nofork. (* Load of ℓ *)
-    { prim_step; apply lookup_insert_eq. }
-    simpl. eapply prim_exec_cons_nofork. (* First redex of let *)
-    { by prim_step. }
-    simpl. eapply prim_exec_cons_nofork. (* Second redex of let *)
-    { by prim_step. }
-    simpl. eapply prim_exec_cons_nofork. (* Comparison ["k" ≤ #0] *)
-    { by prim_step. }
-    rewrite /= bool_decide_false; [|lia].
-    eapply prim_exec_cons_nofork.        (* If *)
-    { by prim_step. }
-    simpl. eapply prim_exec_cons_nofork. (* Decrementing "k" *)
-    { by prim_step. }
-                                         (* CAS *)
-    simpl. eapply (prim_exec_cons_nofork _ _ _ (if: #true then _ else _)).
-    { prim_step; [apply lookup_insert_eq|by left]. }
-    eapply prim_exec_cons_nofork.        (* If *)
-    { by prim_step. }
-    replace (Sn - 1) with (Z.of_nat n) by lia.
-    rewrite insert_insert_eq.
-    apply prim_exec_nil.
+    eapply prim_exec_cons_nofork, prim_exec_nil.
+    apply base_prim_step.
+    destruct σ. simpl.
+    by constructor.
   Qed.
 
   Lemma exec_tick_case_branch e1 v2 σ :
-    prim_exec  (tick_case_branch (λ: <>, e1) v2)%E  σ ((tick e1) v2) σ  [].
+    prim_exec  (tick_case_branch (λ: <>, e1) v2)%E  σ ((Tick e1) v2) σ  [].
   Proof.
     unfold tick_case_branch ; unlock.
     eapply prim_exec_cons_nofork.
@@ -100,6 +53,56 @@ Section Tick_exec.
 
 End Tick_exec.
 
+Lemma tick_counter_decreasing_head_step e σ κ e' σ' efs :
+  head_step e σ κ e' σ' efs →
+  σ'.(tick_counter) ≤ σ.(tick_counter).
+Proof.
+  intros []; try done.
+  match goal with
+    H: tick_counter ?σ' = S ?n |- _ =>
+    destruct σ'
+  end.
+  simpl in *. lia.
+Qed.
+
+Lemma tick_counter_decreasing_prim_step e σ κ e' σ' efs :
+  prim_step e σ κ e' σ' efs →
+  σ'.(tick_counter) ≤ σ.(tick_counter).
+Proof.
+  intros [].
+  by eapply tick_counter_decreasing_head_step.
+Qed.
+
+Lemma tick_counter_decreasing_step t σ κ t' σ' :
+  step (t, σ) κ (t', σ') →
+  σ'.(tick_counter) ≤ σ.(tick_counter).
+Proof.
+  intros []. simplify_eq.
+  by eapply tick_counter_decreasing_prim_step.
+Qed.
+
+Lemma tick_counter_decreasing_erased_step t σ t' σ' :
+  erased_step (t,σ) (t',σ') →
+  σ'.(tick_counter) ≤ σ.(tick_counter).
+Proof.
+  intros [].
+  by eapply tick_counter_decreasing_step.
+Qed.
+
+Lemma tick_counter_decreasing_erased_steps t σ t' σ' :
+  rtc erased_step (t,σ) (t',σ') →
+  σ'.(tick_counter) ≤ σ.(tick_counter).
+Proof.
+  intros Hsteps.
+  remember (t,σ) as cfg eqn:Heq.
+  remember (t',σ') as cfg' eqn:Heq'.
+  replace σ with cfg.2 by rewrite Heq //.
+  replace σ' with cfg'.2 by rewrite Heq' //.
+  clear Heq Heq'.
+  induction Hsteps as [|[] [] [] Hstep Hsteps IH]; first reflexivity.
+  apply tick_counter_decreasing_erased_step in Hstep.
+  simpl in *. lia.
+Qed.
 
 
 (*
@@ -107,8 +110,6 @@ End Tick_exec.
  *)
 
 Section SimulationLemma.
-
-  Context {Hloc : TickCounter}.
 
   Local Ltac exec_tick_success :=
     lazymatch goal with
@@ -135,11 +136,11 @@ Section SimulationLemma.
     tick_then_step_then prim_exec_nil.
 
   Lemma simulation_head_step_success n e1 σ1 κ e2 σ2 efs :
-    σ2 !! ℓ = None →
+    tick_free_expr e1 →
     head_step e1 σ1 κ e2 σ2 efs →
     prim_exec «e1» S«σ1, S n» «e2» S«σ2, n» T«efs».
   Proof.
-    intros Hℓ Hstep.
+    intros Htf Hstep.
     destruct Hstep as
       [ (* RecS *) f x e σ
       | (* PairS *) v1 v2 σ
@@ -161,12 +162,9 @@ Section SimulationLemma.
       | (* CasFailS *) l v1 v2 vl σ  Hbound_l Hneq_vl_v1
       | (* CasSucS *) l v1 v2 σ  Hbound_l
       | (* FaaS *) l i1 i2 σ  Hbound_l
+      | (* TickS *)
       ];
-    simpl_trans;
-    (try (
-      assert (ℓ ≠ l) as I by (by apply lookup_insert_None in Hℓ as [ _ I ]) ;
-      rewrite translationS_insert insert_insert_ne ; last exact I
-    )).
+    simpl_trans; try rewrite translationS_insert.
     (* RecS f x e σ : *)
     - eapply (prim_exec_cons _ _ _ _ _ [] _ _ []).
       + prim_step.
@@ -205,88 +203,94 @@ Section SimulationLemma.
       + exec_tick_success.
     (* AllocS v σ l : *)
     - tick_then_step_then_stop.
-      apply lookup_insert_None ; auto using lookup_translationS_None.
+      rewrite heap_state_set_tick_counter ; auto using lookup_translationS_None.
     (* LoadS l v σ : *)
     - tick_then_step_then_stop.
-      assert (ℓ ≠ l) as I by (intros <- ; rewrite -> Hℓ in * ; discriminate).
-      rewrite lookup_insert_ne ; last exact I.
+      rewrite heap_state_set_tick_counter.
       by apply lookup_translationS_Some.
     (* StoreS l v σ : *)
     - tick_then_step_then_stop.
-      rewrite lookup_insert_ne ; last exact I.
+      rewrite heap_state_set_tick_counter.
       by apply lookup_translationS_is_Some.
     (* CasFailS l v1 v2 vl σ : *)
     - tick_then_step_then_stop.
-      + assert (ℓ ≠ l) as I by (intros <- ; rewrite -> Hℓ in * ; discriminate).
-        rewrite lookup_insert_ne ; last done.
+      + rewrite heap_state_set_tick_counter.
         by apply lookup_translationS_Some.
       + eauto using translationV_injective.
       + by apply vals_cas_compare_safe_translationV.
     (* CasSucS l v1 v2 σ : *)
     - tick_then_step_then_stop.
-      + rewrite lookup_insert_ne ; last exact I.
+      + rewrite heap_state_set_tick_counter.
         by apply lookup_translationS_Some.
       + by apply vals_cas_compare_safe_translationV.
     (* FaaS l i1 i2 σ : *)
     - tick_then_step_then_stop.
-      rewrite lookup_insert_ne ; last exact I.
+      rewrite heap_state_set_tick_counter.
       change (#i1)%V with V« #i1 ».
       by apply lookup_translationS_Some.
+    - by simpl in Htf.
   Qed.
 
   Lemma simulation_prim_step_success n e1 σ1 κ e2 σ2 efs :
-    σ2 !! ℓ = None →
+    tick_free_expr e1 →
     prim_step e1 σ1 κ e2 σ2 efs →
     prim_exec «e1» S«σ1, S n» «e2» S«σ2, n» T«efs».
   Proof.
-    intros Hℓ [ K e1' e2' -> -> H ].
+    intros Htf [ K e1' e2' -> -> H ].
     rewrite 2! translation_fill.
-    by eapply prim_exec_fill, simulation_head_step_success.
+    eapply prim_exec_fill, simulation_head_step_success.
+    - eapply tick_free_expr_fill_e, Htf.
+    - done.
   Qed.
 
   Lemma simulation_step_success n t1 σ1 κ t2 σ2 :
-    σ2 !! ℓ = None →
+    tick_free_config (t1, σ1) →
     step (t1, σ1) κ (t2, σ2) →
     rtc erased_step (T«t1», S«σ1, S n») (T«t2», S«σ2, n»).
   Proof.
-    intros Hℓ Hstep.
+    intros Htc Hstep.
     destruct Hstep as [ e1 σ1_ e2 σ2_ efs t t' E1 E2 Hprimstep ] ;
     injection E1 as -> <- ;
     injection E2 as -> <-.
     repeat rewrite ? fmap_app ? fmap_cons.
-    by eapply exec_frame_singleton_thread_pool, prim_exec_exec,
-       simulation_prim_step_success.
+    eapply exec_frame_singleton_thread_pool, prim_exec_exec,
+      simulation_prim_step_success; last done.
+    destruct Htc as [Htc _].
+    rewrite /= /tick_free_threads Forall_app Forall_cons in Htc.
+    naive_solver.
   Qed.
 
   Lemma simulation_exec_success m n t1 σ1 t2 σ2 :
-    σ2 !! ℓ = None →
+    tick_free_config (t1, σ1) →
     relations.nsteps erased_step m (t1, σ1) (t2, σ2) →
     rtc erased_step (T«t1», S«σ1, m+n») (T«t2», S«σ2, n»).
   Proof.
     make_eq (t1, σ1) as config1 E1.
     make_eq (t2, σ2) as config2 E2.
-    intros Hℓ Hnsteps.
-    revert t1 σ1 E1 ;
+    intros Htf Hnsteps.
+    revert t1 σ1 E1 Htf ;
     induction Hnsteps as [ config | m' config1 (t3, σ3) config2 [κ Hstep] Hsteps IHnsteps ] ;
-    intros t1 σ1 E1.
+    intros t1 σ1 E1 Htf.
     - destruct E2 ; injection E1 as -> ->.
       apply rtc_refl.
     - destruct E2, E1.
       specialize (IHnsteps eq_refl t3 σ3 eq_refl).
-      assert (σ3 !! ℓ = None) as Hℓ3 by (eapply loc_fresh_in_dom_nsteps ; cycle 1 ; eassumption).
+      assert (tick_free_config (t3,σ3)).
+      { by eapply tick_free_step. }
       etrans.
-      + eapply simulation_step_success ; cycle -1 ; eassumption.
-      + apply IHnsteps.
+      + eapply simulation_step_success; eassumption.
+      + by apply IHnsteps.
   Qed.
 
   Lemma simulation_exec_success' m n t1 σ1 t2 σ2 :
-    σ2 !! ℓ = None →
+    tick_free_config (t1, σ1) →
     (m ≤ n)%nat →
     relations.nsteps erased_step m (t1, σ1) (t2, σ2) →
     rtc erased_step (T«t1», S«σ1, n») (T«t2», S«σ2, n-m»).
   Proof.
-    intros Hℓ I.
-    replace #n with #(m + (n-m))%nat ; last (repeat f_equal ; lia).
+    intros Htf I.
+    assert (Hn: n = (m + (n-m))%nat) by (repeat f_equal ; lia).
+    rewrite {1}Hn.
     by apply simulation_exec_success.
   Qed.
 
@@ -303,11 +307,11 @@ Section SimulationLemma.
 
   Lemma active_item_translation_reducible ki v σ m :
     ectx_item_is_active ki →
-    loc_fresh_in_expr ℓ (fill_item ki v) →
+    tick_free_expr (fill_item ki v) →
     reducible (fill_item Ki«ki» V«v») S«σ, m» →
     reducible (fill_item ki v) σ.
   Proof.
-    intros Hactive Hfresh (e2' & σ2' & efs &
+    intros Hactive Htf (e2' & σ2' & efs &
                            [κ Hheadstep % active_item_prim_step_is_head_step]) ;
       last by apply is_active_translationKi.
     make_eq (fill_item Ki«ki» V«v») as e1' Ee1' ; rewrite Ee1' in Hheadstep.
@@ -333,6 +337,7 @@ Section SimulationLemma.
       | (* CasFailS *) l v1 v2 vl σ1  Hbound_l Hneq_vl_v1
       | (* CasSucS *) l v1 v2 σ1  Hbound_l
       | (* FaaS *) l i1 i2 σ1  Hbound_l
+      | (* TickS *)
       ];
     destruct ki ; try contradiction Hactive ; try discriminate Ee1' ;
     injection Ee1' ; clear Ee1' ;
@@ -398,18 +403,19 @@ Section SimulationLemma.
     (* FaaS *)
     - apply lookup_translationS_Some_inv in Hbound_l as (? & ? & -> % eq_sym % translationV_lit_inv).
       by eexhibit_prim_step.
+    - done.
   Qed.
 
   (* assuming the safety of the translated expression,
    * a proof that the original expression is m-safe. *)
 
   Lemma safe_translation__nsafe_here m e σ :
-    loc_fresh_in_expr ℓ e →
+    tick_free_expr e →
     (m > 0)%nat →
     safe «e» S«σ, m» →
     is_Some (to_val e) ∨ reducible e σ.
   Proof.
-    intros Hfresh Im Hsafe.
+    intros Htf Im Hsafe.
     (* case analysis on whether e is a value… *)
     destruct (to_val e) as [ v | ] eqn:Hnotval.
     (* — if e is a value, then we get the result immediately: *)
@@ -439,18 +445,18 @@ Section SimulationLemma.
         eexists _, _, _, _. apply Ectx_step', RecS.
       (* — or e = K[ki[v]] where ki is an active item: *)
       + (* it is enough to show that ki[v] is reducible: *)
-        apply loc_fresh_in_expr_fill_inv in Hfresh ;
+        apply tick_free_expr_fill_e in Htf ;
         rewrite -> translation_fill in Hsafe ; apply safe_fill_inv in Hsafe ;
         apply reducible_fill ;
         clear K.
         (* we deduce the reducibility of ki[v] from that of «ki»[«v»]: *)
         eapply active_item_translation_reducible ; [ done | done | ].
-        (* remind that « ki[v] » = «ki»[tick «v»]: *)
+        (* remind that « ki[v] » = «ki»[Tick «v»]: *)
         rewrite -> translation_fill_item_active in Hsafe ; last done.
-        (* we have that «ki»[tick «v»] reduces to «ki»[«v»]
-         * (m ≥ 1 so ‘tick’ can be run): *)
+        (* we have that «ki»[Tick «v»] reduces to «ki»[«v»]
+         * (m ≥ 1 so ‘Tick’ can be run): *)
         assert (
-          prim_exec (fill_item Ki«ki» (tick V«v»)) S«σ, m»
+          prim_exec (fill_item Ki«ki» (Tick V«v»)) S«σ, m»
                     (fill_item Ki«ki» V«v»)        S«σ, m-1» []
         ) as Hsteps % prim_exec_exec.
         {
@@ -468,15 +474,14 @@ Section SimulationLemma.
         * exact Hred.
   Qed.
   Lemma safe_translation__nsafe m n e σ t2 σ2 e2 :
-    loc_fresh_in_expr ℓ e2 →
-    σ2 !! ℓ = None →
+    tick_free_config ([e],σ) →
     safe «e» S«σ, m» →
     relations.nsteps erased_step n ([e], σ) (t2, σ2) →
     (n < m)%nat →
     e2 ∈ t2 →
     is_Some (to_val e2) ∨ reducible e2 σ2.
   Proof.
-    intros Hℓe Hℓσ Hsafe Hnsteps Inm He2.
+    intros Htf Hsafe Hnsteps Inm He2.
     assert (safe «e2» S«σ2, m-n») as Hsafe2.
     {
       eapply safe_exec.
@@ -485,7 +490,13 @@ Section SimulationLemma.
       - change [«e»] with T«[e]». apply simulation_exec_success' ; [ assumption | lia | assumption ].
     }
     assert (m - n > 0)%nat by lia.
-    by eapply safe_translation__nsafe_here.
+    eapply safe_translation__nsafe_here; [|done..].
+    eapply tick_free_erased_steps in Htf; last by eapply rtc_nsteps_2.
+    destruct Htf as [Htf _].
+    destruct (list_elem_of_split _ _ He2) as (?&?&->).
+    rewrite /tick_free_threads Forall_app Forall_cons in Htf.
+    destruct Htf as (?&?&?).
+    done.
   Qed.
 
   (* assuming the adequacy of the translated expression,
@@ -494,13 +505,13 @@ Section SimulationLemma.
   (* FIXME : this is a weaker result than the adequacy result of Iris,
      where the predicate can also speak about the final state. *)
   Lemma adequate_translation__nadequate_result m n φ e σ t2 σ2 v2 :
-    σ2 !! ℓ = None →
+    tick_free_config ([e],σ) →
     adequate NotStuck «e» S«σ, m» (λ v σ, φ (invtranslationV v)) →
     relations.nsteps erased_step n ([e], σ) (Val v2 :: t2, σ2) →
     (n ≤ m)%nat →
     φ v2.
   Proof.
-    intros Hfresh Hadq Hnsteps Inm.
+    intros Htf Hadq Hnsteps Inm.
     assert (safe «e» S«σ, m») as Hsafe by by eapply safe_adequate.
     replace (φ v2) with ((φ ∘ invtranslationV) (translationV v2))
       by (simpl ; by rewrite invtranslationV_translationV).
@@ -515,31 +526,18 @@ End SimulationLemma. (* we close the section here as we now want to quantify ove
 (* now let’s combine the two results. *)
 
 Lemma adequate_translation__nadequate m φ e σ :
-  (∀ {Hloc : TickCounter}, adequate NotStuck «e» S«σ, m» (λ v σ, φ (invtranslationV v))) →
+  tick_free_config ([e],σ) →
+  adequate NotStuck «e» S«σ, m» (λ v σ, φ (invtranslationV v)) →
   nadequate NotStuck m e σ φ.
 Proof.
-  intros Hadq.
+  intros Htf Hadq.
   split.
   (* (1) adequate result: *)
   - intros n t2 σ2 v2 Hnsteps Inm.
-    (* build a location ℓ which is not in the domain of σ2: *)
-    pose (Hloc := Build_TickCounter (fresh (dom σ2)) : TickCounter).
-    assert (σ2 !! ℓ = None)
-      by (simpl ; eapply (not_elem_of_dom (D:=gset loc)), is_fresh).
     by eapply adequate_translation__nadequate_result.
   (* (2) safety: *)
   - intros n t2 σ2 e2 _ Hnsteps Inm He2.
-    (* build a location ℓ which is fresh in e2 and in the domain of σ2: *)
-    pose (set1 := loc_set_of_expr e2 : gset loc).
-    pose (set2 := dom σ2 : gset loc).
-    pose (Hloc := Build_TickCounter (fresh (set1 ∪ set2)) : TickCounter).
-    eassert (ℓ ∉ set1 ∪ set2) as [Hℓ1 Hℓ2] % not_elem_of_union
-      by (unfold ℓ ; apply is_fresh).
-    assert (loc_fresh_in_expr ℓ e2)
-      by by apply loc_not_in_set_is_fresh_in_expr.
-    assert (σ2 !! ℓ = None)
-      by by (simpl ; eapply (not_elem_of_dom (D:=gset loc))).
-    specialize (Hadq Hloc) as Hsafe % safe_adequate.
+    destruct Hadq as [_ Hsafe].
     by eapply safe_translation__nsafe.
 Qed.
 
